<?xml version="1.0"?>
<!DOCTYPE rdf:RDF [
   <!ENTITY meta   "http://www.openrdf.org/rdf/2009/metadata#" >
   <!ENTITY obj    "http://www.openrdf.org/rdf/2009/object#" >
   <!ENTITY dc     "http://purl.org/dc/elements/1.1/" >
   <!ENTITY owl    "http://www.w3.org/2002/07/owl#" >
   <!ENTITY rdfs   "http://www.w3.org/2000/01/rdf-schema#" >
   <!ENTITY rdf    "http://www.w3.org/1999/02/22-rdf-syntax-ns#" >
   <!ENTITY xsd    "http://www.w3.org/2001/XMLSchema#" >
 ]>
<rdf:RDF xmlns:meta="&meta;" xmlns:obj="&obj;" xmlns:dc="&dc;" xmlns:owl="&owl;" xmlns:rdf="&rdf;" xmlns:rdfs="&rdfs;" xmlns:xsd="&xsd;"
	xml:base="http://www.openrdf.org/rdf/2009/metadata">

	<!-- Annotations -->

	<owl:AnnotationProperty rdf:about="&dc;date" />
	<owl:AnnotationProperty rdf:about="&dc;format" />
	<owl:AnnotationProperty rdf:about="&dc;creator" />

	<!-- Ontology -->

	<owl:Ontology rdf:about="">
		<rdfs:label xml:lang="en">AliBaba Metadata Ontology</rdfs:label>
		<rdfs:comment xml:lang="en">AliBaba Metadata Ontology</rdfs:comment>
		<dc:date rdf:datatype="&xsd;date">2009-06-03</dc:date>
		<dc:format>OWL-Lite</dc:format>
		<dc:creator>James Leigh &lt;james@leighnet.ca&gt;</dc:creator>
		<owl:versionInfo>2.0</owl:versionInfo>
		<owl:imports rdf:resource="http://www.openrdf.org/rdf/2009/object"/>
	</owl:Ontology>

	<!-- Classes -->

	<owl:Class rdf:ID="WebRedirect">
		<rdfs:label xml:lang="en">Web Redirect</rdfs:label>
		<rdfs:comment xml:lang="en">A resource alias.</rdfs:comment>
		<rdfs:isDefinedBy rdf:resource="" />
	</owl:Class>

	<!-- Annotations -->

	<owl:AnnotationProperty rdf:ID="cache-control">
		<rdfs:label xml:lang="en">cache control</rdfs:label>
		<rdfs:comment xml:lang="en">Response directive indicating if entity-bodies can be cached and transformed. This annotation can be placed on classes, properties, and messages.</rdfs:comment>
		<rdfs:isDefinedBy rdf:resource="" />
	</owl:AnnotationProperty>

	<owl:AnnotationProperty rdf:ID="expect">
		<rdfs:label xml:lang="en">expect</rdfs:label>
		<rdfs:comment xml:lang="en">Placed on a method to indicate the HTTP response status code of a successful
response. Possible values include "201-created", "202-accepted",
"205-reset-content", "300-multiple-choices", "301-moved-permanently", and
"302-found".</rdfs:comment>
		<rdfs:isDefinedBy rdf:resource="" />
	</owl:AnnotationProperty>

	<owl:AnnotationProperty rdf:ID="method">
		<rdfs:label xml:lang="en">method</rdfs:label>
		<rdfs:comment xml:lang="en">Placed on messages that should be called for the given HTTP method.</rdfs:comment>
		<rdfs:isDefinedBy rdf:resource="" />
	</owl:AnnotationProperty>

	<owl:AnnotationProperty rdf:ID="operation">
		<rdfs:label xml:lang="en">operation</rdfs:label>
		<rdfs:comment xml:lang="en">Placed on properties or messages that should be called when the given request parameter name is sent without a value.</rdfs:comment>
		<rdfs:isDefinedBy rdf:resource="" />
	</owl:AnnotationProperty>

	<owl:AnnotationProperty rdf:ID="parameter">
		<rdfs:label xml:lang="en">parameter</rdfs:label>
		<rdfs:comment xml:lang="en">Placed on message properties that should be populated with request GET query parameters.</rdfs:comment>
		<rdfs:isDefinedBy rdf:resource="" />
	</owl:AnnotationProperty>

	<owl:AnnotationProperty rdf:ID="rel">
		<rdfs:label xml:lang="en">rel</rdfs:label>
		<rdfs:comment xml:lang="en">Placed on properties or messages and describes the relationship from the domain to the property range or message response.</rdfs:comment>
		<rdfs:isDefinedBy rdf:resource="" />
	</owl:AnnotationProperty>

	<owl:AnnotationProperty rdf:ID="title">
		<rdfs:label xml:lang="en">title</rdfs:label>
		<rdfs:comment xml:lang="en">Labels the property range or message response such that it can be used as identification within a human-readable menu.</rdfs:comment>
		<rdfs:isDefinedBy rdf:resource="" />
	</owl:AnnotationProperty>

	<owl:AnnotationProperty rdf:ID="transform">
		<rdfs:label xml:lang="en">transform</rdfs:label>
		<rdfs:comment xml:lang="en">The messages that should be used to transform the
parameter or response.</rdfs:comment>
		<rdfs:isDefinedBy rdf:resource="" />
	</owl:AnnotationProperty>

	<owl:AnnotationProperty rdf:ID="type">
		<rdfs:label xml:lang="en">type</rdfs:label>
		<rdfs:comment xml:lang="en">Space separated list of media types that may reside in this property range or message response.</rdfs:comment>
		<rdfs:isDefinedBy rdf:resource="" />
	</owl:AnnotationProperty>

	<!-- Properties -->

	<owl:ObjectProperty rdf:ID="redirect">
		<rdf:type rdf:resource="&owl;FunctionalProperty" />
		<rdfs:label xml:lang="en">redirect</rdfs:label>
		<rdfs:comment xml:lang="en">Indicates this resource resides temporarily under a different URI.</rdfs:comment>
		<rdfs:isDefinedBy rdf:resource="" />
		<rdfs:domain rdf:resource="#WebRedirect" />
	</owl:ObjectProperty>

	<owl:DatatypeProperty rdf:ID="mediaType">
		<rdf:type rdf:resource="&owl;FunctionalProperty" />
		<rdfs:label xml:lang="en">media type</rdfs:label>
		<rdfs:comment xml:lang="en">The media type of the resource, including any parameters.</rdfs:comment>
		<rdfs:isDefinedBy rdf:resource="" />
		<rdfs:range rdf:resource="&xsd;string" />
	</owl:DatatypeProperty>

	<owl:DatatypeProperty rdf:ID="contentMD5">
		<rdf:type rdf:resource="&owl;FunctionalProperty" />
		<rdfs:label xml:lang="en">content MD5</rdfs:label>
		<rdfs:comment xml:lang="en">The MD5 hash (as defined by HTTP 1.1) of the Web content for this resource.</rdfs:comment>
		<rdfs:isDefinedBy rdf:resource="" />
		<rdfs:range rdf:resource="&xsd;string" />
	</owl:DatatypeProperty>

	<owl:DatatypeProperty rdf:ID="contentEncoding">
		<rdf:type rdf:resource="&owl;FunctionalProperty" />
		<rdfs:label xml:lang="en">content encoding</rdfs:label>
		<rdfs:comment xml:lang="en">A value of "gzip" indicates the content of this resource has been compressed.</rdfs:comment>
		<rdfs:isDefinedBy rdf:resource="" />
		<rdfs:range rdf:resource="&xsd;string" />
	</owl:DatatypeProperty>

</rdf:RDF>
