<?xml version="1.0"?>
<!DOCTYPE rdf:RDF [
   <!ENTITY obj "http://www.openrdf.org/rdf/2009/object#" >
   <!ENTITY dc     "http://purl.org/dc/elements/1.1/" >
   <!ENTITY owl    "http://www.w3.org/2002/07/owl#" >
   <!ENTITY rdfs   "http://www.w3.org/2000/01/rdf-schema#" >
   <!ENTITY rdf    "http://www.w3.org/1999/02/22-rdf-syntax-ns#" >
   <!ENTITY xsd    "http://www.w3.org/2001/XMLSchema#" >
 ]>
<rdf:RDF xmlns:obj="&obj;" xmlns:dc="&dc;" xmlns:owl="&owl;" xmlns:rdf="&rdf;" xmlns:rdfs="&rdfs;" xmlns:xsd="&xsd;"
	xml:base="http://www.openrdf.org/rdf/2009/object">

	<!-- Ontology -->

	<owl:Ontology rdf:about="">
		<rdfs:label xml:lang="en">Object</rdfs:label>
		<dc:title xml:lang="en">AliBaba Object Ontology</dc:title>
		<dc:date rdf:datatype="&xsd;date">2009-03-02</dc:date>
		<dc:format>OWL-Lite</dc:format>
		<dc:creator>James Leigh &lt;james@leighnet.ca&gt;</dc:creator>
		<owl:versionInfo>2.0</owl:versionInfo>
	</owl:Ontology>

	<!-- Classes -->

	<owl:Class rdf:ID="Message">
		<rdfs:label xml:lang="en">Message</rdfs:label>
		<rdfs:comment xml:lang="en">The base class for all messages.</rdfs:comment>
		<rdfs:isDefinedBy rdf:resource="" />
	</owl:Class>

	<owl:Class rdf:ID="TupleResult">
		<rdfs:label xml:lang="en">Tuple Result</rdfs:label>
		<rdfs:comment xml:lang="en">An ordered result set of binding names and their values.</rdfs:comment>
		<rdfs:isDefinedBy rdf:resource="" />
	</owl:Class>

	<owl:Class rdf:ID="GraphResult">
		<rdfs:label xml:lang="en">Graph Result</rdfs:label>
		<rdfs:comment xml:lang="en">A consumable graph stream.</rdfs:comment>
		<rdfs:isDefinedBy rdf:resource="" />
	</owl:Class>

	<!-- Annotations -->

	<owl:AnnotationProperty rdf:ID="className">
		<rdfs:label xml:lang="en">class name</rdfs:label>
		<rdfs:comment xml:lang="en">The Java class name that should be used for this annotation, concept, behaviour, or message.</rdfs:comment>
		<rdfs:isDefinedBy rdf:resource="" />
	</owl:AnnotationProperty>

	<owl:AnnotationProperty rdf:ID="name">
		<rdfs:label xml:lang="en">name</rdfs:label>
		<rdfs:comment xml:lang="en">The Java property or method name that should be used for this property or message.</rdfs:comment>
		<rdfs:isDefinedBy rdf:resource="" />
	</owl:AnnotationProperty>

	<owl:AnnotationProperty rdf:ID="componentType">
		<rdfs:label xml:lang="en">component type</rdfs:label>
		<rdfs:comment xml:lang="en">Indicates the class of the list members.</rdfs:comment>
		<rdfs:isDefinedBy rdf:resource="" />
	</owl:AnnotationProperty>

	<owl:AnnotationProperty rdf:ID="localized">
		<rdfs:label xml:lang="en">localized</rdfs:label>
		<rdfs:comment xml:lang="en">Used on properties with language tagged literals. A value of "functional" requires at most one literal per language tag, whereas a value of "multivalued" may contain many values within a language tag.</rdfs:comment>
		<rdfs:isDefinedBy rdf:resource="" />
	</owl:AnnotationProperty>

	<owl:AnnotationProperty rdf:ID="readOnly">
		<rdfs:label xml:lang="en">read only</rdfs:label>
		<rdfs:comment xml:lang="en">Used on properties that cannot be changed through an object. A value of "true" indicates that the property value should not be modified through an object interface.</rdfs:comment>
		<rdfs:isDefinedBy rdf:resource="" />
	</owl:AnnotationProperty>

	<owl:AnnotationProperty rdf:ID="precedes">
		<rdfs:label xml:lang="en">precedes</rdfs:label>
		<rdfs:comment xml:lang="en">This method precedes the given methods if they are used together.</rdfs:comment>
		<rdfs:isDefinedBy rdf:resource="" />
	</owl:AnnotationProperty>

	<owl:AnnotationProperty rdf:ID="matches">
		<rdfs:label xml:lang="en">matches</rdfs:label>
		<rdfs:comment xml:lang="en">Any resource with a URI matching an entire given expression is an instance of this class. Expressions ending with '*' are matched against the prefix. Expressions starting with '/' are matched from the beginning of the path (if hierarchical). This annotation should be used in an anonymous class to assign properties and messages by URI patterns.</rdfs:comment>
		<rdfs:isDefinedBy rdf:resource="" />
	</owl:AnnotationProperty>

	<!-- Message Properties -->

	<owl:ObjectProperty rdf:ID="target">
		<rdf:type rdf:resource="&owl;FunctionalProperty" />
		<rdfs:label xml:lang="en">target</rdfs:label>
		<rdfs:comment xml:lang="en">The receiver of this message.</rdfs:comment>
		<rdfs:isDefinedBy rdf:resource="" />
		<rdfs:domain rdf:resource="#Message" />
	</owl:ObjectProperty>

	<owl:ObjectProperty rdf:ID="objectResponse">
		<rdfs:label xml:lang="en">object response</rdfs:label>
		<rdfs:comment xml:lang="en">The return value of this message.</rdfs:comment>
		<rdfs:isDefinedBy rdf:resource="" />
		<rdfs:domain rdf:resource="#Message" />
	</owl:ObjectProperty>

	<owl:DatatypeProperty rdf:ID="literalResponse">
		<rdfs:label xml:lang="en">literal response</rdfs:label>
		<rdfs:comment xml:lang="en">The return value of this message.</rdfs:comment>
		<rdfs:isDefinedBy rdf:resource="" />
		<rdfs:domain rdf:resource="#Message" />
	</owl:DatatypeProperty>

	<owl:ObjectProperty rdf:ID="functionalObjectResponse">
		<rdf:type rdf:resource="&owl;FunctionalProperty" />
		<rdfs:label xml:lang="en">functional object response</rdfs:label>
		<rdfs:comment xml:lang="en">Single return value of this message.</rdfs:comment>
		<rdfs:isDefinedBy rdf:resource="" />
		<rdfs:subPropertyOf rdf:resource="#objectResponse" />
		<rdfs:domain rdf:resource="#Message" />
	</owl:ObjectProperty>

	<owl:DatatypeProperty rdf:ID="functionalLiteralResponse">
		<rdf:type rdf:resource="&owl;FunctionalProperty" />
		<rdfs:label xml:lang="en">functional literal response</rdfs:label>
		<rdfs:comment xml:lang="en">Single return value of this message.</rdfs:comment>
		<rdfs:isDefinedBy rdf:resource="" />
		<rdfs:subPropertyOf rdf:resource="#literalResponse" />
		<rdfs:domain rdf:resource="#Message" />
	</owl:DatatypeProperty>

	<owl:AnnotationProperty rdf:ID="triggeredBy">
		<rdfs:label xml:lang="en">triggered by</rdfs:label>
		<rdfs:comment xml:lang="en">Placed on methods that should be executed when statements are added with the
given predicate. The methods must response with owl:Nothing and take no parameters or have a
single parameter matching the range of the given property.</rdfs:comment>
		<rdfs:isDefinedBy rdf:resource="" />
	</owl:AnnotationProperty>

	<owl:AnnotationProperty rdf:ID="imports">
		<rdfs:label xml:lang="en">imports</rdfs:label>
		<rdfs:comment xml:lang="en">A Class that maybe referenced locally in this method or trigger. This annotation should be used in conjunction with the java and groovy annotations.</rdfs:comment>
		<rdfs:isDefinedBy rdf:resource="" />
	</owl:AnnotationProperty>

	<owl:AnnotationProperty rdf:ID="java">
		<rdfs:label xml:lang="en">java</rdfs:label>
		<rdfs:comment xml:lang="en">The block of Java code for this method or trigger. The variable msg is available in the code block and refers to the individual message instance that is being evaluated (different for each call). The individual message will contain any declared parameters (message properties) and the current response. Calling the method proceed on the individual message will cause any other methods to be evaluated with this message and updating the current response. The implementation will implement the declared target class and the interface RDFObject. The methods getResource and getObjectConnection are available to access the underlying RDF store.</rdfs:comment>
		<rdfs:isDefinedBy rdf:resource="" />
	</owl:AnnotationProperty>

	<owl:AnnotationProperty rdf:ID="groovy">
		<rdfs:label xml:lang="en">groovy</rdfs:label>
		<rdfs:comment xml:lang="en">The block of Groovy code for this method or trigger. The variable msg is available in the code block and refers to the individual message instance that is being evaluated (different for each call). The individual message will contain any declared parameters (message properties) and the current response. Calling the method proceed on the individual message will cause any other methods to be evaluated with this message and updating the current response. The implementation will implement the declared target class and the interface RDFObject. The methods getResource and getObjectConnection are available to access the underlying RDF store.</rdfs:comment>
		<rdfs:isDefinedBy rdf:resource="" />
	</owl:AnnotationProperty>

	<owl:AnnotationProperty rdf:ID="sparql">
		<rdfs:label xml:lang="en">sparql</rdfs:label>
		<rdfs:comment xml:lang="en">Named SPARQL queries should be placed in this annotation on methods that
should respond with this query. The method parameters must have the @name annotation. In addition to the parameters, the variable "self" will be bound to the message target. It is recommended to use the '$' prefix for explicitly bound variables (as in $self) and '?' for all other variables.</rdfs:comment>
		<rdfs:isDefinedBy rdf:resource="" />
	</owl:AnnotationProperty>

	<owl:AnnotationProperty rdf:ID="xslt">
		<rdfs:label xml:lang="en">xslt</rdfs:label>
		<rdfs:comment xml:lang="en">XSLT markup or XSLT URL should
be placed in this annotation on methods that should respond with this
style sheet transformation. All but one parameter must have the @name
annotation. In addition to the parameters, the parameter "self" will be bound to the message target URI as a string.</rdfs:comment>
		<rdfs:isDefinedBy rdf:resource="" />
	</owl:AnnotationProperty>

	<!-- Messages -->

	<owl:Class rdf:ID="proceed">
		<rdfs:label xml:lang="en">proceed</rdfs:label>
		<rdfs:comment xml:lang="en">Called to allow the message to proceed to the next implementation method.</rdfs:comment>
		<rdfs:isDefinedBy rdf:resource="" />
		<rdfs:subClassOf rdf:resource="#Message"/>
		<rdfs:subClassOf>
			<owl:Restriction>
				<owl:onProperty rdf:resource="&obj;target" />
				<owl:allValuesFrom rdf:resource="#Message" />
			</owl:Restriction>
		</rdfs:subClassOf>
		<rdfs:subClassOf>
			<owl:Restriction>
				<owl:onProperty rdf:resource="&obj;objectResponse" />
				<owl:allValuesFrom rdf:resource="&owl;Nothing" />
			</owl:Restriction>
		</rdfs:subClassOf>
	</owl:Class>

</rdf:RDF>
