<?xml version="1.0"?>
<!DOCTYPE rdf:RDF [
   <!ENTITY dc     "http://purl.org/dc/elements/1.1/" >
   <!ENTITY owl    "http://www.w3.org/2002/07/owl#" >
   <!ENTITY rdfs   "http://www.w3.org/2000/01/rdf-schema#" >
   <!ENTITY rdf    "http://www.w3.org/1999/02/22-rdf-syntax-ns#" >
   <!ENTITY xsd    "http://www.w3.org/2001/XMLSchema#" >
   <!ENTITY prov   "http://www.w3.org/ns/prov#" >
   <!ENTITY audit  "http://www.openrdf.org/rdf/2012/auditing#" >
 ]>
<rdf:RDF xmlns:dc="&dc;" xmlns:owl="&owl;" xmlns:rdf="&rdf;"
	xmlns:rdfs="&rdfs;" xmlns:xsd="&xsd;" xmlns:aud="&audit;"
	xml:base="http://www.openrdf.org/rdf/2012/auditing">

	<!-- Ontology -->

	<owl:Ontology rdf:about="">
		<rdfs:label xml:lang="en">Auditing Repository</rdfs:label>
		<dc:title xml:lang="en">AliBaba Auditing Repository Ontology</dc:title>
		<dc:date rdf:datatype="&xsd;date">2012-11-13</dc:date>
		<dc:format>OWL-Lite</dc:format>
		<dc:creator>James Leigh &lt;james@3roundstones.com&gt;</dc:creator>
		<owl:versionInfo>2.0</owl:versionInfo>
	</owl:Ontology>

	<!-- Classes -->

	<owl:Class rdf:ID="RecentBundle">
		<rdfs:label xml:lang="en">Recent Bundle</rdfs:label>
		<rdfs:comment xml:lang="en">A rolling set of recent activity bundles.</rdfs:comment>
		<rdfs:isDefinedBy rdf:resource="" />
		<rdfs:subClassOf rdf:resource="&prov;Bundle" />
	</owl:Class>

	<owl:Class rdf:ID="ObsoleteBundle">
		<rdfs:label xml:lang="en">Obsolete Bundle</rdfs:label>
		<rdfs:comment xml:lang="en">An activity bundle that does not contribute to the current state of any entity.</rdfs:comment>
		<rdfs:isDefinedBy rdf:resource="" />
		<rdfs:subClassOf rdf:resource="&prov;Bundle" />
	</owl:Class>

	<!-- Properties -->

	<owl:ObjectProperty rdf:ID="without">
		<rdfs:label xml:lang="en">without</rdfs:label>
		<rdfs:comment xml:lang="en">Triple that was deleted as part of the process that generate this entity.</rdfs:comment>
		<rdfs:isDefinedBy rdf:resource="" />
		<rdfs:domain rdf:resource="&prov;Entity" />
		<rdfs:range rdf:resource="&rdf;Statement" />
	</owl:ObjectProperty>

	<!-- Properties -->

	<owl:ObjectProperty rdf:ID="with">
		<rdfs:label xml:lang="en">with</rdfs:label>
		<rdfs:comment xml:lang="en">Triple that was inserted as part of the process that generate this entity.</rdfs:comment>
		<rdfs:isDefinedBy rdf:resource="" />
		<rdfs:domain rdf:resource="&prov;Entity" />
		<rdfs:range rdf:resource="&rdf;Statement" />
	</owl:ObjectProperty>

</rdf:RDF>
