<?xml version="1.0"?>
<!DOCTYPE rdf:RDF [
   <!ENTITY http   "http://www.openrdf.org/rdf/2009/httpobject#" >
   <!ENTITY obj    "http://www.openrdf.org/rdf/2009/object#" >
   <!ENTITY dc     "http://purl.org/dc/elements/1.1/" >
   <!ENTITY owl    "http://www.w3.org/2002/07/owl#" >
   <!ENTITY rdfs   "http://www.w3.org/2000/01/rdf-schema#" >
   <!ENTITY rdf    "http://www.w3.org/1999/02/22-rdf-syntax-ns#" >
   <!ENTITY xsd    "http://www.w3.org/2001/XMLSchema#" >
 ]>
<rdf:RDF xmlns:http="&http;" xmlns:obj="&obj;" xmlns:dc="&dc;" xmlns:owl="&owl;" xmlns:rdf="&rdf;" xmlns:rdfs="&rdfs;" xmlns:xsd="&xsd;"
	xml:base="http://www.openrdf.org/rdf/2009/httpobject">

	<!-- Ontology -->

	<owl:Ontology rdf:about="">
		<rdfs:label xml:lang="en">HTTP Object</rdfs:label>
		<dc:title xml:lang="en">AliBaba HTTP Object Ontology</dc:title>
		<dc:date rdf:datatype="&xsd;date">2010-02-06</dc:date>
		<dc:format>OWL-Lite</dc:format>
		<dc:creator>James Leigh &lt;james@leighnet.ca&gt;</dc:creator>
		<owl:versionInfo>2.0</owl:versionInfo>
		<owl:imports rdf:resource="http://www.openrdf.org/rdf/2009/object"/>
	</owl:Ontology>

	<!-- Classes -->

	<owl:Class rdf:ID="Realm">
		<rdfs:label xml:lang="en">Realm</rdfs:label>
		<rdfs:comment xml:lang="en">A security context.</rdfs:comment>
		<rdfs:isDefinedBy rdf:resource="" />
	</owl:Class>

	<owl:Class rdf:ID="DigestRealm">
		<rdfs:label xml:lang="en">Digest Realm</rdfs:label>
		<rdfs:comment xml:lang="en">A security context that uses digest access authentication.</rdfs:comment>
		<rdfs:isDefinedBy rdf:resource="" />
	</owl:Class>

	<owl:Class rdf:ID="Credential">
		<rdfs:label xml:lang="en">Credential</rdfs:label>
		<rdfs:comment xml:lang="en">A credential for authentication.</rdfs:comment>
		<rdfs:isDefinedBy rdf:resource="" />
	</owl:Class>

	<!-- Annotations -->

	<owl:AnnotationProperty rdf:ID="cache-control">
		<rdfs:label xml:lang="en">cache control</rdfs:label>
		<rdfs:comment xml:lang="en">Response directive indicating if entity-bodies can be cached and transformed. This annotation can be placed on classes, properties, and messages.</rdfs:comment>
		<rdfs:isDefinedBy rdf:resource="" />
	</owl:AnnotationProperty>

	<owl:AnnotationProperty rdf:ID="encoding">
		<rdfs:label xml:lang="en">encoding</rdfs:label>
		<rdfs:comment xml:lang="en">Placed on a method to indicate the desired HTTP response content encoding.</rdfs:comment>
		<rdfs:isDefinedBy rdf:resource="" />
	</owl:AnnotationProperty>

	<owl:AnnotationProperty rdf:ID="expect">
		<rdfs:label xml:lang="en">expect</rdfs:label>
		<rdfs:comment xml:lang="en">Placed on a method to indicate the HTTP response status code of a successful
response. Possible values include "201-created", "202-accepted",
"205-reset-content", "300-multiple-choices", "301-moved-permanently", and
"302-found".</rdfs:comment>
		<rdfs:isDefinedBy rdf:resource="" />
	</owl:AnnotationProperty>

	<owl:AnnotationProperty rdf:ID="header">
		<rdfs:label xml:lang="en">header</rdfs:label>
		<rdfs:comment xml:lang="en">Placed on message properties that should be populated with request GET headers.</rdfs:comment>
		<rdfs:isDefinedBy rdf:resource="" />
	</owl:AnnotationProperty>

	<owl:AnnotationProperty rdf:ID="method">
		<rdfs:label xml:lang="en">method</rdfs:label>
		<rdfs:comment xml:lang="en">Placed on messages that should be called for the given HTTP method.</rdfs:comment>
		<rdfs:isDefinedBy rdf:resource="" />
	</owl:AnnotationProperty>

	<owl:AnnotationProperty rdf:ID="operation">
		<rdfs:label xml:lang="en">operation</rdfs:label>
		<rdfs:comment xml:lang="en">Placed on properties or messages that should be called when the given request query parameter name is sent without a value.</rdfs:comment>
		<rdfs:isDefinedBy rdf:resource="" />
	</owl:AnnotationProperty>

	<owl:AnnotationProperty rdf:ID="parameter">
		<rdfs:label xml:lang="en">parameter</rdfs:label>
		<rdfs:comment xml:lang="en">Placed on message properties that should be populated with request GET query parameters.</rdfs:comment>
		<rdfs:isDefinedBy rdf:resource="" />
	</owl:AnnotationProperty>

	<owl:AnnotationProperty rdf:ID="realm">
		<rdfs:label xml:lang="en">realm</rdfs:label>
		<rdfs:comment xml:lang="en">The Realm used to secure members of this class or use of this message.</rdfs:comment>
		<rdfs:isDefinedBy rdf:resource="" />
	</owl:AnnotationProperty>

	<owl:AnnotationProperty rdf:ID="rel">
		<rdfs:label xml:lang="en">rel</rdfs:label>
		<rdfs:comment xml:lang="en">Placed on properties or messages and describes the relationship from the domain to the property range or message response.</rdfs:comment>
		<rdfs:isDefinedBy rdf:resource="" />
	</owl:AnnotationProperty>

	<owl:AnnotationProperty rdf:ID="title">
		<rdfs:label xml:lang="en">title</rdfs:label>
		<rdfs:comment xml:lang="en">Labels the property range or message response such that it can be used as identification within a human-readable menu.</rdfs:comment>
		<rdfs:isDefinedBy rdf:resource="" />
	</owl:AnnotationProperty>

	<owl:AnnotationProperty rdf:ID="transform">
		<rdfs:label xml:lang="en">transform</rdfs:label>
		<rdfs:comment xml:lang="en">The messages that should be used to transform the
parameter or response.</rdfs:comment>
		<rdfs:isDefinedBy rdf:resource="" />
	</owl:AnnotationProperty>

	<owl:AnnotationProperty rdf:ID="type">
		<rdfs:label xml:lang="en">type</rdfs:label>
		<rdfs:comment xml:lang="en">Space separated list of media types that may reside in this property range or message response.</rdfs:comment>
		<rdfs:isDefinedBy rdf:resource="" />
	</owl:AnnotationProperty>

	<!-- Properties -->

	<owl:DatatypeProperty rdf:ID="realmAuth">
		<rdf:type rdf:resource="&owl;FunctionalProperty" />
		<rdfs:label xml:lang="en">realm auth</rdfs:label>
		<rdfs:comment xml:lang="en">A string to be displayed to users so they know which username and
password to use. This string should contain at least the name of the host
performing the authentication and might additionally indicate the
collection of users who might have access. An example might be
"registered_users@gotham.news.com".</rdfs:comment>
		<rdfs:isDefinedBy rdf:resource="" />
		<rdfs:domain rdf:resource="#DigestRealm" />
		<rdfs:range rdf:resource="&xsd;string" />
	</owl:DatatypeProperty>

	<owl:DatatypeProperty rdf:ID="origin">
		<rdfs:label xml:lang="en">origin</rdfs:label>
		<rdfs:comment xml:lang="en">Identifies the security context that caused the user agent to initiate an HTTP request.</rdfs:comment>
		<rdfs:isDefinedBy rdf:resource="" />
		<rdfs:domain rdf:resource="#DigestRealm" />
		<rdfs:range rdf:resource="&xsd;string" />
	</owl:DatatypeProperty>

	<owl:ObjectProperty rdf:ID="credential">
		<rdfs:label xml:lang="en">credential</rdfs:label>
		<rdfs:comment xml:lang="en">Credentials that can be used in this Realm.</rdfs:comment>
		<rdfs:isDefinedBy rdf:resource="" />
		<rdfs:domain rdf:resource="#DigestRealm" />
		<rdfs:range rdf:resource="#Credential" />
	</owl:ObjectProperty>

	<owl:DatatypeProperty rdf:ID="name">
		<rdf:type rdf:resource="&owl;FunctionalProperty" />
		<rdfs:label xml:lang="en">name</rdfs:label>
		<rdfs:comment xml:lang="en">A unique username within this Realm to identify the credential.</rdfs:comment>
		<rdfs:isDefinedBy rdf:resource="" />
		<rdfs:domain rdf:resource="#Credential" />
		<rdfs:range rdf:resource="&xsd;string" />
	</owl:DatatypeProperty>

	<owl:DatatypeProperty rdf:ID="algorithm">
		<rdf:type rdf:resource="&owl;FunctionalProperty" />
		<rdfs:label xml:lang="en">algorithm</rdfs:label>
		<rdfs:comment xml:lang="en">Must have the value "MD5".</rdfs:comment>
		<rdfs:isDefinedBy rdf:resource="" />
		<rdfs:domain rdf:resource="#Credential" />
		<rdfs:range rdf:resource="&xsd;string" />
	</owl:DatatypeProperty>

	<owl:DatatypeProperty rdf:ID="encoded">
		<rdf:type rdf:resource="&owl;FunctionalProperty" />
		<rdfs:label xml:lang="en">encoded</rdfs:label>
		<rdfs:comment xml:lang="en">The HA1 MD5 hash value of the username:realm:password.</rdfs:comment>
		<rdfs:isDefinedBy rdf:resource="" />
		<rdfs:domain rdf:resource="#Credential" />
		<rdfs:range rdf:resource="&xsd;hexBinary" />
	</owl:DatatypeProperty>

</rdf:RDF>
